

# Практика 10 ДМ

№1

$$xy \vee (x \neg y \vee \neg xy) = xy \vee x \neg y \vee \neg xy = x \vee \neg xy = x \vee y$$

$$xy \rightarrow x = \neg(xy) \vee x = \neg x \vee \neg y \vee x = 1$$

$$f = (\neg x \rightarrow z) \rightarrow \neg(\neg y \rightarrow \neg x) = (x \vee z) \rightarrow (\neg y \wedge x) = \neg x \wedge \neg z \vee \neg y \wedge x$$

$$\text{СДНФ: } \neg x \neg z y \vee \neg x \neg z \neg y \vee x \neg y z \vee z \neg y \neg z$$

$$f = x(yz \rightarrow xy) = x(\neg(y \wedge z) \vee x \wedge y) = x \wedge \neg y \vee x \wedge \neg z \vee x \wedge y = x(\neg y \vee \neg z \vee y)$$

СКНФ:

$$(\neg x \vee \neg y \vee \neg z) \wedge (\neg x \vee \neg y \vee z) \wedge (\neg x \vee y \vee \neg z) \wedge (\neg x \vee y \vee z) \wedge (x \vee y \vee z) \wedge (x \vee \neg y \vee z)$$

$$f = x(yz \rightarrow xy)$$

1. Сохраняет 0  $f(0, \dots, 0) = 0$
2. Сохраняет 1  $f(1, \dots, 1) = 1$
3. Монотонная
4. Самодвойственная

№2

Линейная  $f =$

#0

1. no
2. yes
3. yes
4. no
5.  $f = 1$

#1

1. yes
2. no
3. yes
4.  $f(\neg 0) = f(1) = 0 = f(0)$
5.  $f = 0$

#^

1. yes
2. no
3. no
4.  $f(\neg x; \neg y) = \neg f(x; y)$

5.  $f = xy$

# $\vee$

1. yes

2. yes

3. yes

4.  $f(\neg x \vee \neg y) = \neg f(x \vee y)$

5.  $f = x + y + xy$

# $\neg$

1. no

2. no

3. no

4.  $f(\neg x) = \neg f(x)$

5.  $f = \neg x$

# $\rightarrow$

1. no

2. yes

3. no

4.  $f(\neg x; \neg y) = \neg f(x; y)$

5.  $f = x + xy + 1$

# $\downarrow$

1. no

2. no

3. no

4.  $f(\neg x; \neg y) = \neg f(x; y)$

5.  $f = y + x + xy$

# $\leftrightarrow$

1. no

2. yes

3. no

4.  $f(\neg x \leftrightarrow \neg y) = \neg f(x \leftrightarrow y)$

5.  $f = 1 + x + y$

# $|$

1. yes

2. yes

3. yes

4.  $f(\neg x | \neg y) = \neg f(x | y)$

5.  $f = 1 + xy$

№3

# $\neg$

1. no

2. no

3. no

4. yes

5. no

# $\cap$

1. yes

2. yes

3. yes

4. no

5. no

{ $\neg, \wedge$ } - базис

№4

1.  $f(11110001)$

x y z f

0 0 0 1

0 0 1 1

0 1 0 1

0 1 1 1

1 0 0 0

1 0 1 0

1 1 0 0

1 1 1 1

СДНФ:  $f : (\neg x \wedge \neg y \wedge \neg z) \vee (\neg x \wedge \neg y \wedge z) \vee (\neg x \wedge y \wedge z) \vee (x \wedge y \wedge z)$

СКНФ:  $f : (\neg x \vee y \vee z) \wedge (\neg x \vee y \vee \neg z) \wedge (\neg x \vee \neg y \vee z)$

2.  $f(00010101)$

x y z f

0 0 0 0

0 0 1 0

0 1 0 0

0 1 1 1

1 0 0 0

1 0 1 1

1 1 0 0

1 1 1 1

$CDH\Phi : f : (\neg xyz \vee xy\neg z \vee xyz)$

$CKH\Phi : f : (x \vee y \vee z) \wedge (x \vee y \vee \neg z) \wedge (x \vee \neg y \vee z) \wedge (\neg x \vee y \vee z) \wedge (\neg x \vee y \vee \neg z)$

№5

1.  $f = (--0-01--) f \in M$

x y z f

0 0 0 0

0 0 1 0

0 1 0 0

0 1 1 0

1 0 0 0

1 0 1 1

1 1 0 1

1 1 1 1

$f = (00000111)$

2.  $g = (--0-01--) g \in L$

x y z f

0 0 0

0 0 1

0 1 0

0 1 1 1

1 0 0

1 0 1 0

1 1 0 1

1 1 1 0

$g = (---1-010)$

3.  $h = (1-10--1-) h \in S$

x y z f

0 0 0 1

0 0 1 0

0 1 0 1

0 1 1 0

1 0 0 1

1 0 1 0

1 1 0 1

1 1 1 0

$h = (10101010)$

№6

$f=(10100001)$

$g=(00111100)$

$\{f; g\}$

x y z f g

0 0 0 1 0

0 0 1 0 0

0 1 0 1 1

0 1 1 0 1

1 0 0 0 1

1 0 1 0 1

1 1 0 0 0

1 1 1 1 0